Auto/Lib/HList.lean
@@ -1,0 +1,13 @@
+namespace Auto
+
+inductive HList (β : α → Sort _) : List α → Sort _
+  | nil  : HList β .nil
+  | cons : (x : β ty) → HList β tys → HList β (ty :: tys)
+
+def HList.getD {β : α → Sort _} {ty : α} (default : β ty) :
+  {tys : List α} → HList β tys → (n : Nat) → β (tys.getD n ty)
+  | .nil, .nil,       _       => default
+  | .(_), .cons a _,  0       => a
+  | .(_), .cons _ as, .succ n => HList.getD default as n
+
+end Auto
