Auto/Lib/ListExtra.lean
@@ -1,0 +1,30 @@
+namespace Auto
+
+-- This function is slow and is not meant to be used in
+--   computation. It's main use is in the pushs_pops theorems
+def List.ofFun (f : Nat → α) (n : Nat) : List α :=
+  match n with
+  | 0 => .nil
+  | .succ n' => f 0 :: ofFun (fun n => f (.succ n)) n'
+
+theorem List.ofFun_length (f : Nat → α) (n : Nat) :
+  (List.ofFun f n).length = n := by
+  revert f; induction n <;> intros f
+  case zero => rfl
+  case succ n IH => dsimp [ofFun]; rw [IH]
+
+theorem List.ofFun_get?_eq_some (f : Nat → α) (n m : Nat) (h : n > m) :
+  (List.ofFun f n).get? m = .some (f m) := by
+  revert f n; induction m <;> intros f n h
+  case zero =>
+    cases n
+    case zero => cases h
+    case succ n => rfl
+  case succ m IH =>
+    cases n
+    case zero => cases h
+    case succ n =>
+      let h' := Nat.le_of_succ_le_succ h
+      dsimp [ofFun, List.get?]; rw [IH (fun n => f (.succ n)) _ h']
+
+end Auto
