Auto/Lib/ToExprExtra.lean
@@ -50,4 +50,13 @@ instance {α : Type u} [ToSortLevel.{u}] [ToExpr α] : ToExpr (Array α) :=
   { toExpr     := fun as => mkApp2 (mkConst ``Array.mk [lvl]) type (toExpr as.toList),
     toTypeExpr := mkApp (mkConst ``Array [lvl]) type }
 
+-- Used when the elements of a container are already expressions
+-- For example, consider the ordinary
+--   `l₁ := toExpr (a : List Nat)`
+--   `l₂ := (a : List Nat).map toExpr`
+-- We require that `toExpr (self:=instExprToExprId (.const ``Nat [])) l₂ ≝ l₁`
+-- It is obvious that this shouldn't be marked as an `instance`
+def instExprToExprId (ty : Expr) : ToExpr Expr :=
+  { toExpr := id, toTypeExpr := ty}
+
 end Auto
